@prefix owl: <http://www.w3.org/2002/07/owl#> .
@prefix rdf: <http://www.w3.org/1999/02/22-rdf-syntax-ns#> .
@prefix rdfs: <http://www.w3.org/2000/01/rdf-schema#> .
@prefix vann: <http://purl.org/vocab/vann/> .
@prefix schema: <http://schema.org/> .

schema: a owl:Ontology ;
	vann:preferredNamespacePrefix "schema" ; 
	rdfs:label "Schema.org" ; 
	rdfs:comment "An ontology developed by Google, Yahoo!, Microsoft and others to describe people, places, and things commonly found on the web." 
. 

schema:rangeIncludes a rdf:Property ;
	rdfs:comment """
		A Class that is known to be in the range of this Property.  This is a modeling construct invented by the Schema.org
		consortium as an alternative to rdfs:range.  It allows one to identify one of many possible values for a property
		instead of specifying exactly one class (or a complicated equivalent class).
	""" ;
	rdfs:domain rdf:Property ;
	rdfs:range rdfs:Class 
.

schema:domainIncludes a rdf:Property ;
	rdfs:comment """
		A Class that is known to be in the domain of this Property.  This is a modeling construct invented by the Schema.org
		consortium as an alternative to rdfs:domain.  It allows one to identify one of many possible classes that can have
		the specified property instead of defining exactly one class (or a complicated equivalent class).
	""" ;
	rdfs:domain rdf:Property ;
	rdfs:range rdfs:Class
.		