@prefix kcs: <http://www.konig.io/ns/kcs/> .
@prefix kol: <http://www.konig.io/ns/kol/> .
@prefix owl: <http://www.w3.org/2002/07/owl#> .
@prefix sh: <http://www.w3.org/ns/shacl#> .
@prefix rdfs: <http://www.w3.org/2000/01/rdf-schema#> .
@prefix vann: <http://purl.org/vocab/vann/> .
@prefix xsd: <http://www.w3.org/2001/XMLSchema#> .
@prefix cs: <http://purl.org/vocab/changeset/schema#> .
@prefix rdf: <http://www.w3.org/1999/02/22-rdf-syntax-ns#> .

kcs: a owl:Ontology ;
	rdfs:label "Konig ChangeSet" ;
	rdfs:comment """This vocabulary extends the <em>defacto</em> standard 
	  <a href="http://vocab.org/changeset/">ChangeSet ontology</a>
    so that <code>additions</code> and <code>removals</code> can be expressed as graphs rather than collections
    of <code>rdf:Statement</code> instances, and it introduces the notion of a <em>reference</em> graph
    which is used to identify blank nodes that have been modified.</p>""" ;
	vann:preferredNamespacePrefix "kcs" 
	.
	
kcs:reference a owl:ObjectProperty ;
	rdfs:comment """A collection of statements that uniquely identify the initial state of any blank nodes
	  that are modified by the <code>ChangeSet</code>.  
		<p>For each blank node undergoing a change, the statements must provide enough information to distinguish that node
		from any other node in the starting state of the target graph.  This information could consist of a complete 
		enumeration of all the node's properties, values of functional or inverse functional properties, etc.</p>""" ;
	rdfs:domain cs:ChangeSet ;
	rdfs:range kol:Graph
	.
	
kcs:trace a owl:ObjectProperty ;
  rdfs:comment """A statement which helps trace the identity of a blank node.  The collection of all
    such statements within the <code>ChangeSet</code> forms the <code>reference</code> graph which
    contains enough information to distinguish each blank node from any other blank node.""" ;
  rdfs:domain cs:ChangeSet ;
  rdfs:range rdf:Statement 
  .	
	
kcs:add a owl:ObjectProperty ;
	rdfs:comment "A graph of statements to be added to the target resource." ;
	rdfs:domain cs:ChangeSet ;
	rdfs:range kol:Graph
	.
	
kcs:remove a owl:ObjectProperty ;	
	rdfs:comment "A graph of statements to be removed from the target resource." ;
	rdfs:domain cs:ChangeSet ;
	rdfs:range kol:Graph
	.

kcs:source a owl:ObjectProperty ;
	rdfs:comment """A Graph that provides a complete description of the initial state of the 
		<code>subjectOfChange</code>.""" ;
	rdfs:domain cs:ChangeSet ;
	rdfs:range kol:Graph 
	.
	
kcs:target a owl:ObjectProperty ;
	rdfs:comment """A Graph that provides a complete description of the final state of the 
		<code>subjectOfChange</code> after it has been mutated by the ChangeSet."""	;
	rdfs:domain cs:ChangeSet ;
	rdfs:range kol:Graph
	.
	