@prefix kol: <http://www.konig.io/ns/kol/> .
@prefix owl: <http://www.w3.org/2002/07/owl#> .
@prefix sh: <http://www.w3.org/ns/shacl#> .
@prefix rdfs: <http://www.w3.org/2000/01/rdf-schema#> .
@prefix vann: <http://purl.org/vocab/vann/> .
@prefix xsd: <http://www.w3.org/2001/XMLSchema#> .

kol: a owl:Ontology ;
	rdfs:label "Konig Ontology Language" ;
	rdfs:comment """Provides terms that extend OWL and SHACL.
		<p>A description of this ontology in Turtle syntax is available at 
		<a href="http://www.konig.io/ns/kol/.ttl">http://www.konig.io/ns/kol/.ttl</a></p>""" ;
	vann:preferredNamespacePrefix "kol"
	.

kol:Graph a owl:Class ;
	rdfs:comment "A set of statements which collectively form a (possibly disconnected) graph."
	.

kol:JsonSchemaSpecification a owl:Class ;
	rdfs:comment "A document containing a JSON Schema specification"
	.
	
kol:AvroSchemaSpecification a owl:Class ;
	rdfs:comment "A document containing an Avro Schema specification"
	.	

kol:LogicalShape a owl:Class ;
	rdfs:subClassOf sh:Shape ;
	rdfs:comment """
		A Shape that provides a logical model for the Class identified as the <code>scopeClass</code>.  
		A <code>LogicalShape</code> lists all the known properties of the <code>scopeClass</code>.  
		It does not prescribe a <code>valueShape</code> for any related entities."""
	.
	
kol:ForeignKeyProperty 
	rdfs:subClassOf rdfs:Property ;
	rdfs:comment """
		A property whose value is a foreign key that uniquely identifies some related entity.
		That is, the value is identical to the value of some inverse functional property of the 
		related entity.  This style of expressing a relationship is discouraged
		because it does not follow linked data principles.  However, it is useful for expressing relationships
		defined by an RDBMS schema or a REST API that does not adhere to linked data principles.
	"""
	.
	
kol:equivalentObjectProperty a owl:ObjectProperty ;
	rdfs:comment """
		A property that expresses the same relationship as this ForeignKeyProperty, but as an ObjectProperty
		whose value is the related entity (as opposed to the value of a unique key that identifies the related entity).
	""" ;
	rdfs:domain kol:ForeignKeyProperty ;
	rdfs:range owl:ObjectProperty
	.
	
kol:referencedClass a owl:ObjectPropery ;
	rdfs:comment "The OWL Class for the type of entity referenced by the foreign key" ;
	rdfs:domain kol:ForeignKeyProperty ;
	rdfs:range owl:Class
	.
			
	
kol:keyProperty a owl:ObjectProperty ;
	rdfs:comment """
		The property on the related entity whose value is the same as the value of this ForeignKeyProperty.
	""" ;
	rdfs:domain kol:ForeignKeyProperty ;
	rdfs:range 	owl:InverseFunctionalProperty
	.
	

kol:uniqueIn	a owl:ObjectProperty ;
	rdfs:domain rdfs:Datatype ;
	rdfs:range rdfs:Resource ;
	rdfs:comment "A property which asserts that values of the subject Datatype are unique within some entity that serves as a namespace."
	.
	
kol:valueUniqueIn a owl:ObjectProperty ;
	rdfs:domain sh:PropertyConstraint ;	
	rdfs:range rdfs:Resource ;
	rdfs:comment "Asserts that values of the given property are unique within some entity that serves as a namespace."
	.
	
kol:tableName a owl:DatatypeProperty ;
	rdfs:domain sh:Shape ;
	rdfs:range	xsd:string ;	
	rdfs:comment "The preferred name for an RDBMS table that contains instances of the subject Shape" .
	
kol:columnName a owl:DatatypeProperty ;
	rdfs:domain sh:PropertyConstraint ;
	rdfs:range xsd:string ;
	rdfs:comment "The preferred name for an RDBMS column that contains values of the <code>predicate</code>" .
		

kol:propertyOf a owl:ObjectProperty ;
	rdfs:domain sh:PropertyConstraint ;
	rdfs:range sh:Shape ;
	owl:inverseOf sh:property ;
	rdfs:comment "The <code>Shape</code> to which the subject <code>PropertyConstraint</code> applies" .
		
kol:knownIndividual a owl:ObjectProperty ;
	rdfs:domain sh:PropertyConstraint ;
	rdfs:range owl:NamedIndividual ;
	rdfs:comment "A named individual that is known to be a possible value for the property."
	.		
	
kol:mediaTypeBaseName a owl:DatatypeProperty ;	
	rdfs:domain sh:Shape ;
	rdfs:range xsd:string ;
	rdfs:comment "The base name for the vendor-specific media type associated with this Shape"
	.
	
kol:jsonSchemaRendition	a owl:ObjectProperty ;
	rdfs:domain sh:Shape ;
	rdfs:range kol:JsonSchemaSpecification ;
	rdfs:comment "The JSON Schema specification corresponding to this Shape"
	.
	
kol:avroSchemaRendition a owl:ObjectProperty ;
	rdfs:domain sh:Shape ;
	rdfs:range kol:JsonSchemaSpecification ;
	rdfs:comment "The Avro Schema specification corresponding to this Shape"
	.
		
kol:equivalentRelationalShape a owl:ObjectProperty ;
	rdfs:comment """
		A Shape equivalent to this one, but where object properties are replaced by		
		ForeignKeyProperties where possible.
	""" ;
	rdfs:domain sh:Shape ;
	rdfs:range sh:Shape
	.
		