@prefix kol: <http://www.konig.io/ns/kol/> .
@prefix owl: <http://www.w3.org/2002/07/owl#> .
@prefix sh: <http://www.w3.org/ns/shacl#> .
@prefix rdfs: <http://www.w3.org/2000/01/rdf-schema#> .
@prefix vann: <http://purl.org/vocab/vann/> .
@prefix xsd: <http://www.w3.org/2001/XMLSchema#> .

kol: a owl:Ontology ;
	rdfs:label "Konig Ontology Language" ;
	rdfs:comment """Provides terms that extend OWL and SHACL.
		<p>A description of this ontology in Turtle syntax is available at 
		<a href="http://www.konig.io/ns/kol/.ttl">http://www.konig.io/ns/kol/.ttl</a></p>""" ;
	vann:preferredNamespacePrefix "kol"
	.


kol:Graph a owl:Class ;
	rdfs:comment "A set of statements which collectively form a (possibly disconnected) graph."
	.

kol:LogicalShape a owl:Class ;
	rdfs:subClassOf sh:Shape ;
	rdfs:comment """
		A Shape that provides a logical model for the Class identified as the <code>scopeClass</code>.  
		A <code>LogicalShape</code> lists all the known properties of the <code>scopeClass</code>.  
		It does not prescribe a <code>valueShape</code> for any related entities."""
	.
	
kol:ForeignKey a owl:Class ;
	rdfs:subClassOf sh:Constraint ;
	rdfs:comment "A foreign key constraint on a Shape." .

kol:uniqueIn	a owl:ObjectProperty ;
	rdfs:domain rdfs:Datatype ;
	rdfs:range rdfs:Resource ;
	rdfs:comment "A property which asserts that values of the subject Datatype are unique within some entity that serves as a namespace."
	.
	
kol:valueUniqueIn a owl:ObjectProperty ;
	rdfs:domain sh:PropertyConstraint ;	
	rdfs:range rdfs:Resource ;
	rdfs:comment "Asserts that values of the given property are unique within some entity that serves as a namespace."
	.
	
kol:tableName a owl:DatatypeProperty ;
	rdfs:domain sh:Shape ;
	rdfs:range	xsd:string ;	
	rdfs:comment "The preferred name for an RDBMS table that contains instances of the subject Shape" .
	
kol:columnName a owl:DatatypeProperty ;
	rdfs:domain sh:PropertyConstraint ;
	rdfs:range xsd:string ;
	rdfs:comment "The preferred name for an RDBMS column that contains values of the <code>predicate</code>" .
	
kol:foreignKey a owl:ObjectProperty, owl:FunctionalProperty ;
	rdfs:domain kol:ForeignKey ;
	rdfs:range rdf:List ;
	rdfs:comment """
		A property that lists the predicate(s) which form a foreign key.  
		The value of this property is a List so that composite keys can be supported.  The type of entity
		referenced by the foreign key is given by the <code>kol:referencedClass</code> property.  
		The corresponding primary key on the referenced class is given by the <code>kol:referencedKey</code>. """ .	
		
kol:referencedClass a owl:ObjectProperty, owl:FunctionalProperty ;
	rdfs:domain kol:ForeignKey ;
	rdfs:range rdfs:Class ;
	rdfs:comment "The type of entity referenced by the foreign key." .
	
kol:referencedKey a owl:ObjectProperty, owl:FunctionalProperty ;
	rdfs:domain kol:ForeignKey ;
	rdfs:range rdf:List ;
	rdfs:comment """
		A property that lists the predicate(s) on the referenced entity corresponding to 
		the foreign keys on the source entity.  The value of this property is a List so that
		composite keys can be supported.  The elements of the List are in one-to-one correspondence with
		the elements of the <code>foreignKey</code> List.""" .
		
kol:equivalentSemanticProperty a owl:ObjectProperty, owl:FunctionalProperty ;
	rdfs:domain kol:ForeignKey ;
	rdfs:range rdf:Property ;
	rdfs:comment "An equivalent semantic property that expresses the same relationship as this foreign key." .
	
kol:propertyOf a owl:ObjectProperty ;
	rdfs:domain sh:PropertyConstraint ;
	rdfs:range sh:Shape ;
	owl:inverseOf sh:property ;
	rdfs:comment "The <code>Shape</code> to which the subject <code>PropertyConstraint</code> applies" .
		
			
		